((t (t 1+)) 0)
(define (t f)
  (lambda (x) (f (f (f x)))) )

((t (t 1+)) 0) => 
((t (lambda (x) (1+ (1+ (1+ x))))) 0) =>
(((lambda (x) ((lambda (x) (1+ (1+ (1+ x)))) ((lambda (x) (1+ (1+ (1+ x)))) ((lambda (x) (1+ (1+ (1+ x)))) x)))) ) 0) =>
(((lambda (x) (1+ (1+ (1+ x)))) ((lambda (x) (1+ (1+ (1+ x)))) 3) )) => 9


(((t t) 1+) 0) =>
((((lambda (x) ((lambda (f) (lambda (x) (f (f (f x)))) ) ((lambda (f) (lambda (x) (f (f (f x)))) ) ((lambda (f) (lambda (x) (f (f (f x)))) ) x))))) 1+) 0) =>
( ( ( ((lambda (f) (lambda (x) (f (f (f x)))) ) ((lambda (f) (lambda (x) (f (f (f x)))) ) ((lambda (f) (lambda (x) (f (f (f x)))) ) 1+))))) 0) =>
( ( ( ((lambda (f) (lambda (x) (f (f (f x)))) ) ((lambda (f) (lambda (x) (f (f (f x)))) ) ( (lambda (x) (1+ (1+ (1+ x)))) ) )))) 0) =>
( ( ( ((lambda (f) (lambda (x) (f (f (f x)))) ) ( (lambda (x) ((lambda (x) (1+ (1+ (1+ x)))) ((lambda (x) (1+ (1+ (1+ x)))) ((lambda (x) (1+ (1+ (1+ x)))) x)))) )))) 0) =>
( ( ( ( (lambda (x) ((lambda (x) ((lambda (x) (1+ (1+ (1+ x)))) ((lambda (x) (1+ (1+ (1+ x)))) ((lambda (x) (1+ (1+ (1+ x)))) x))) ) ((lambda (x) ((lambda (x) (1+ (1+ (1+ x)))) ((lambda (x) (1+ (1+ (1+ x)))) ((lambda (x) (1+ (1+ (1+ x)))) x))) ) ((lambda (x) ((lambda (x) (1+ (1+ (1+ x)))) ((lambda (x) (1+ (1+ (1+ x)))) ((lambda (x) (1+ (1+ (1+ x)))) x))) ) x)))) ))) 0) =>
( ( ( ( ( ( (1+ (1+ (1+ x)))) ((lambda (x) (1+ (1+ (1+ x)))) ((lambda (x) (1+ (1+ (1+ x)))) x))) ) ((lambda (x) ((lambda (x) (1+ (1+ (1+ x)))) ((lambda (x) (1+ (1+ (1+ x)))) ((lambda (x) (1+ (1+ (1+ x)))) x))) ) ((lambda (x) ((lambda (x) (1+ (1+ (1+ x)))) ((lambda (x) (1+ (1+ (1+ x)))) ((lambda (x) 3) )) ) )))) )) => 27

( ( (lambda (f) (lambda (x) (f (f (f x)))) ) 1+) 0)